coq/LLVMGen/Correctness_MExpr.v
@@ -42,6 +42,7 @@ Require Import Vellvm.InterpreterCFG.
 Require Import Vellvm.TopLevelRefinements.
 Require Import Vellvm.TypToDtyp.
 Require Import Vellvm.LLVMEvents.
+Require Import Vellvm.Denotation_Theory.
 
 Require Import Ceres.Ceres.
 
